ocaml/fstar-lib/generated/FStar_Interactive_Incremental.ml
@@ -534,7 +534,7 @@ let (format_code :
             FStar_Parser_AST.drange = uu___; FStar_Parser_AST.quals = uu___1;
             FStar_Parser_AST.attrs = uu___2;
             FStar_Parser_AST.interleaved = uu___3;_}::uu___4 ->
-            FStar_Pervasives_Native.Some (l, FStar_Pervasives_Native.None) in
+            FStar_Pervasives_Native.Some l in
       let parse_result = parse_code maybe_lang code in
       match parse_result with
       | FStar_Parser_ParseIt.IncrementalFragment
